tuned proofs; tuned whitespace;

thys/Separation_Logic_Imperative_HOL/Examples/Hash_Table.thy
@@ -1,6 +1,6 @@
 section "Hash-Tables"
 theory Hash_Table
-  imports "../../Collections/Lib/HashCode" "../Sep_Main"
+imports "../../Collections/Lib/HashCode" "../Sep_Main"
 begin
 
 subsection {* Datatype *}
@@ -9,114 +9,109 @@ subsubsection {* Definition *}
 
 datatype ('k, 'v) hashtable = HashTable "('k \<times> 'v) list array" nat
 
-primrec the_array :: "('k, 'v) hashtable \<Rightarrow> ('k \<times> 'v) list array" where
-  "the_array (HashTable a _) = a"
+primrec the_array :: "('k, 'v) hashtable \<Rightarrow> ('k \<times> 'v) list array"
+  where "the_array (HashTable a _) = a"
 
-primrec the_size :: "('k, 'v) hashtable \<Rightarrow> nat" where
-  "the_size (HashTable _ n) = n" 
+primrec the_size :: "('k, 'v) hashtable \<Rightarrow> nat"
+  where "the_size (HashTable _ n) = n"
+
 
 subsubsection {* Storable on Heap *}
 
-fun
-  hs_encode :: "('k::countable, 'v::countable) hashtable \<Rightarrow> nat"
-  where
-  "hs_encode (HashTable a n) = to_nat (n, a)"
+fun hs_encode :: "('k::countable, 'v::countable) hashtable \<Rightarrow> nat"
+  where "hs_encode (HashTable a n) = to_nat (n, a)"
 
 instance hashtable :: (countable, countable) countable
 proof (rule countable_classI[of "hs_encode"])
-  case goal1 thus ?case
-    by (cases x, cases y, auto)
+  fix x y :: "('a, 'b) hashtable"
+  assume "hs_encode x = hs_encode y"
+  then show "x = y" by (cases x, cases y) auto
 qed
 
 instance hashtable :: (heap, heap) heap ..
 
-subsection {* Assertions *}
 
+subsection {* Assertions *}
 
 subsubsection {* Assertion for Hashtable *}
 
-definition ht_table 
-  :: "('k::heap \<times> 'v::heap) list list \<Rightarrow> ('k, 'v) hashtable \<Rightarrow> assn" 
-  where
-  "ht_table l ht = (the_array ht) \<mapsto>\<^sub>a l"
+definition ht_table :: "('k::heap \<times> 'v::heap) list list \<Rightarrow> ('k, 'v) hashtable \<Rightarrow> assn"
+  where "ht_table l ht = (the_array ht) \<mapsto>\<^sub>a l"
 
-definition ht_size :: "'a list list \<Rightarrow> nat \<Rightarrow> bool" where
-  "ht_size l n \<equiv> n = listsum (map length l)"
+definition ht_size :: "'a list list \<Rightarrow> nat \<Rightarrow> bool"
+  where "ht_size l n \<equiv> n = listsum (map length l)"
 
 definition ht_hash :: "('k::hashable \<times> 'v) list list \<Rightarrow> bool" where
-  "ht_hash l 
-  \<equiv> \<forall>i<length l. \<forall>x\<in>set (l!i). 
-      bounded_hashcode_nat (length l) (fst x) = i"
+  "ht_hash l \<equiv> \<forall>i<length l. \<forall>x\<in>set (l!i).
+    bounded_hashcode_nat (length l) (fst x) = i"
 
 definition ht_distinct :: "('k \<times> 'v) list list \<Rightarrow> bool" where
   "ht_distinct l \<equiv> \<forall>i<length l. distinct (map fst (l!i))"
 
 
-definition is_hashtable 
-  :: "('k::{heap,hashable} \<times> 'v::heap) list list 
-    \<Rightarrow> ('k, 'v) hashtable \<Rightarrow> assn" 
-  where 
-  "is_hashtable l ht = 
-  (the_array ht \<mapsto>\<^sub>a l) * 
-  \<up>(ht_size l (the_size ht) 
-    \<and> ht_hash l 
-    \<and> ht_distinct l 
+definition is_hashtable :: "('k::{heap,hashable} \<times> 'v::heap) list list
+    \<Rightarrow> ('k, 'v) hashtable \<Rightarrow> assn"
+where
+  "is_hashtable l ht =
+  (the_array ht \<mapsto>\<^sub>a l) *
+  \<up>(ht_size l (the_size ht)
+    \<and> ht_hash l
+    \<and> ht_distinct l
     \<and> 1 < length l)"
 
-lemma is_hashtable_prec:
-  "precise is_hashtable"
-  apply rule
+lemma is_hashtable_prec: "precise is_hashtable"
+  apply (rule preciseI)
   unfolding is_hashtable_def
-  by (auto simp add: preciseD[OF snga_prec])
-    
+  apply (auto simp add: preciseD[OF snga_prec])
+  done
+
 text {* These rules are quite useful for automated methods, to avoid unfolding
-  of definitions, that might be used folded in other lemmas, 
-  like induction hypothesis. However, they show in some sense a possibility for 
-  modularization improvement, as it should be enough to show an implication 
+  of definitions, that might be used folded in other lemmas,
+  like induction hypothesis. However, they show in some sense a possibility for
+  modularization improvement, as it should be enough to show an implication
   and know that the @{text "nth"} and @{text "len"} operations do not change
   the heap. *}
 lemma ht_array_nth_rule[sep_heap_rules]:
-    "i<length l \<Longrightarrow> <is_hashtable l ht> 
-      Array.nth (the_array ht) i 
+    "i<length l \<Longrightarrow> <is_hashtable l ht>
+      Array.nth (the_array ht) i
       <\<lambda>r. is_hashtable l ht * \<up>(r = l!i)>"
   unfolding is_hashtable_def
   by sep_auto
 
 lemma ht_array_length_rule[sep_heap_rules]:
-    "<is_hashtable l ht> 
-      Array.len (the_array ht) 
+    "<is_hashtable l ht>
+      Array.len (the_array ht)
       <\<lambda>r. is_hashtable l ht * \<up>(r = length l)>"
   unfolding is_hashtable_def
   by sep_auto
+
 
 subsection {* New *}
 
 subsubsection {* Definition *}
 
-definition ht_new_sz 
-  :: "nat \<Rightarrow> ('k::{heap,hashable}, 'v::heap) hashtable Heap" 
-  where
-  "ht_new_sz n \<equiv> do { let l = replicate n []; 
+definition ht_new_sz :: "nat \<Rightarrow> ('k::{heap,hashable}, 'v::heap) hashtable Heap"
+where
+  "ht_new_sz n \<equiv> do { let l = replicate n [];
   a \<leftarrow> Array.of_list l;
   return (HashTable a 0) }"
 
 
-definition ht_new :: "('k::{heap,hashable}, 'v::heap) hashtable Heap" 
+definition ht_new :: "('k::{heap,hashable}, 'v::heap) hashtable Heap"
   where "ht_new \<equiv> ht_new_sz (def_hashmap_size TYPE('k))"
 
 
 subsubsection {* Complete Correctness *}
 
 lemma ht_hash_replicate[simp, intro!]: "ht_hash (replicate n [])"
-  apply (induct n) 
+  apply (induct n)
   apply (auto simp add: ht_hash_def)
   apply (case_tac i)
   apply auto
   done
 
-lemma ht_distinct_replicate[simp, intro!]: 
-  "ht_distinct (replicate n [])"
-  apply (induct n) 
+lemma ht_distinct_replicate[simp, intro!]: "ht_distinct (replicate n [])"
+  apply (induct n)
   apply (auto simp add: ht_distinct_def)
   apply (case_tac i)
   apply auto
@@ -126,8 +121,7 @@ lemma ht_size_replicate[simp, intro!]: "ht_size (replicate n []) 0"
   by (simp add: ht_size_def)
 
  -- "We can't create hash tables with a size of zero"
-lemma complete_ht_new_sz:
-  shows "1 < n \<Longrightarrow> <emp> ht_new_sz n <is_hashtable (replicate n [])>"
+lemma complete_ht_new_sz: "1 < n \<Longrightarrow> <emp> ht_new_sz n <is_hashtable (replicate n [])>"
   apply (unfold ht_new_sz_def)
   apply (simp del: replicate.simps)
   apply (rule bind_rule)
@@ -137,24 +131,24 @@ lemma complete_ht_new_sz:
   done
 
 lemma complete_ht_new:
-  shows 
-  "<emp> 
-     ht_new::('k::{heap,hashable}, 'v::heap) hashtable Heap 
+  "<emp>
+     ht_new::('k::{heap,hashable}, 'v::heap) hashtable Heap
    <is_hashtable (replicate (def_hashmap_size TYPE('k)) [])>"
   unfolding ht_new_def
   by (simp add: complete_ht_new_sz[OF def_hashmap_size])
+
 
 subsection {* Lookup *}
 
 subsubsection {* Definition *}
 
-fun ls_lookup :: "'k \<Rightarrow> ('k \<times> 'v) list \<Rightarrow> 'v option" where
+fun ls_lookup :: "'k \<Rightarrow> ('k \<times> 'v) list \<Rightarrow> 'v option"
+where
   "ls_lookup x [] = None" |
   "ls_lookup x ((k, v) # l) = (if x = k then Some v else ls_lookup x l)"
 
-definition ht_lookup 
-  :: "'k \<Rightarrow> ('k::{heap,hashable}, 'v::heap) hashtable \<Rightarrow> 'v option Heap"
-  where
+definition ht_lookup :: "'k \<Rightarrow> ('k::{heap,hashable}, 'v::heap) hashtable \<Rightarrow> 'v option Heap"
+where
   "ht_lookup x ht = do {
     m \<leftarrow> Array.len (the_array ht);
     let i = bounded_hashcode_nat m x;
@@ -162,11 +156,12 @@ definition ht_lookup
     return (ls_lookup x l)
   }"
 
+
 subsubsection {* Complete Correctness *}
 
-lemma complete_ht_lookup: 
-  "<is_hashtable l ht> ht_lookup x ht 
-     <\<lambda>r. is_hashtable l ht * 
+lemma complete_ht_lookup:
+  "<is_hashtable l ht> ht_lookup x ht
+     <\<lambda>r. is_hashtable l ht *
         \<up>(r = ls_lookup x (l!(bounded_hashcode_nat (length l) x))) >"
   apply (cases ht)
   apply (clarsimp simp: is_hashtable_def)
@@ -179,98 +174,96 @@ lemma complete_ht_lookup:
   apply (simp add: bounded_hashcode_nat_bounds)
   apply (rule norm_pre_pure_rule)
   apply (rule return_cons_rule)
-  by simp
+  apply simp
+  done
 
 text {* Alternative, more automatic proof *}
 lemma complete_ht_lookup_alt_proof:
-  "<is_hashtable l ht> ht_lookup x ht 
-    <\<lambda>r. is_hashtable l ht * 
+  "<is_hashtable l ht> ht_lookup x ht
+    <\<lambda>r. is_hashtable l ht *
       \<up>(r = ls_lookup x (l!(bounded_hashcode_nat (length l) x)))>"
   unfolding is_hashtable_def ht_lookup_def
   apply (cases ht)
   apply (sep_auto simp: bounded_hashcode_nat_bounds)
   done
 
+
 subsection {* Update *}
 
 subsubsection {* Definition *}
 
-fun ls_update :: "'k \<Rightarrow> 'v \<Rightarrow> ('k \<times> 'v) list \<Rightarrow> (('k \<times> 'v) list \<times> bool)" where
+fun ls_update :: "'k \<Rightarrow> 'v \<Rightarrow> ('k \<times> 'v) list \<Rightarrow> (('k \<times> 'v) list \<times> bool)"
+where
   "ls_update k v [] = ([(k, v)], False)" |
   "ls_update k v ((l, w) # ls) = (
-    if k = l then 
-      ((k, v) # ls, True) 
-    else 
+    if k = l then
+      ((k, v) # ls, True)
+    else
       (let r = ls_update k v ls in ((l, w) # fst r, snd r))
   )"
 
-definition abs_update 
+definition abs_update
   :: "'k::hashable \<Rightarrow> 'v \<Rightarrow> ('k \<times> 'v) list list \<Rightarrow> ('k \<times> 'v) list list"
   where
-  "abs_update k v l = 
-    l[bounded_hashcode_nat (length l) k 
+  "abs_update k v l =
+    l[bounded_hashcode_nat (length l) k
       := fst (ls_update k v (l ! bounded_hashcode_nat (length l) k))]"
 
-lemma ls_update_snd_set:
-  "snd (ls_update k v l) \<longleftrightarrow> k \<in> set (map fst l)"
+lemma ls_update_snd_set: "snd (ls_update k v l) \<longleftrightarrow> k \<in> set (map fst l)"
   by (induct l rule: ls_update.induct) simp_all
 
-lemma ls_update_fst_set:
-  "set (fst (ls_update k v l)) \<subseteq> insert (k, v) (set l)"
-  apply (induct l rule: ls_update.induct) 
+lemma ls_update_fst_set: "set (fst (ls_update k v l)) \<subseteq> insert (k, v) (set l)"
+  apply (induct l rule: ls_update.induct)
   apply simp
-  by (auto simp add: Let_def)
+  apply (auto simp add: Let_def)
+  done
 
-lemma ls_update_fst_map_set:
-  "set (map fst (fst (ls_update k v l))) = insert k (set (map fst l))"
-  apply (induct l rule: ls_update.induct) 
+lemma ls_update_fst_map_set: "set (map fst (fst (ls_update k v l))) = insert k (set (map fst l))"
+  apply (induct l rule: ls_update.induct)
   apply simp
-  by (auto simp add: Let_def)
+  apply (auto simp add: Let_def)
+  done
 
-lemma ls_update_distinct: "distinct (map fst l) 
-  \<Longrightarrow> distinct (map fst (fst (ls_update k v l)))"
+lemma ls_update_distinct: "distinct (map fst l) \<Longrightarrow> distinct (map fst (fst (ls_update k v l)))"
 proof (induct l rule: ls_update.induct)
-  case goal1 thus ?case by simp
+  case 1 thus ?case by simp
 next
-  case goal2 show ?case
+  case (2 k v l w ls) show ?case
   proof (cases "k = l")
     case True
-    with goal2 show ?thesis by simp
+    with 2 show ?thesis by simp
   next
     case False
-    with goal2 have d: "distinct (map fst (fst (ls_update k v ls)))"
+    with 2 have d: "distinct (map fst (fst (ls_update k v ls)))"
       by simp
-    from goal2(2) have "l \<notin> set (map fst ls)" by simp
+    from 2(2) have "l \<notin> set (map fst ls)" by simp
     with False have "l \<notin> set (map fst (fst (ls_update k v ls)))"
-      apply (simp only: ls_update_fst_map_set) by simp
+      by (simp only: ls_update_fst_map_set) simp
     with d False show ?thesis by (simp add: Let_def)
   qed
 qed
 
-lemma ls_update_length: "length (fst (ls_update k v l)) 
+lemma ls_update_length: "length (fst (ls_update k v l))
   = (if (k \<in> set (map fst l)) then length l else Suc (length l))"
-  apply (induct l rule: ls_update.induct)
-  by (auto simp add: Let_def)
+  by (induct l rule: ls_update.induct) (auto simp add: Let_def)
 
 lemma ls_update_length_snd_True:
   "snd (ls_update k v l) \<Longrightarrow> length (fst (ls_update k v l)) = length l"
   by (simp add: ls_update_length ls_update_snd_set)
 
 lemma ls_update_length_snd_False:
-  "\<not> snd (ls_update k v l) 
-  \<Longrightarrow> length (fst (ls_update k v l)) = Suc (length l)"
+  "\<not> snd (ls_update k v l) \<Longrightarrow> length (fst (ls_update k v l)) = Suc (length l)"
   by (simp add: ls_update_length ls_update_snd_set)
 
 
-
-definition ht_upd 
-  :: "'k \<Rightarrow> 'v 
-    \<Rightarrow> ('k::{heap,hashable}, 'v::heap) hashtable 
-    \<Rightarrow> ('k, 'v) hashtable Heap" 
+definition ht_upd
+  :: "'k \<Rightarrow> 'v
+    \<Rightarrow> ('k::{heap,hashable}, 'v::heap) hashtable
+    \<Rightarrow> ('k, 'v) hashtable Heap"
   where
   "ht_upd k v ht = do {
-      m \<leftarrow> Array.len (the_array ht); 
-      let i = bounded_hashcode_nat m k; 
+      m \<leftarrow> Array.len (the_array ht);
+      let i = bounded_hashcode_nat m k;
       l \<leftarrow> Array.nth (the_array ht) i;
       let l = ls_update k v l;
       Array.upd i (fst l) (the_array ht);
@@ -278,65 +271,68 @@ definition ht_upd
       return (HashTable (the_array ht) n)
     }"
 
+
 subsubsection {* Complete Correctness *}
+
 lemma ht_hash_update:
   assumes "ht_hash ls"
   shows "ht_hash (abs_update k v ls)"
   unfolding ht_hash_def abs_update_def
-proof (intro allI ballI impI, simp)
-  case goal1 show ?case
-    proof (cases "i = bounded_hashcode_nat (length ls) k")
+  apply (intro allI ballI impI)
+  apply simp
+  subgoal premises prems for i x
+  proof (cases "i = bounded_hashcode_nat (length ls) k")
+    case True
+    note i = True
+    show ?thesis
+    proof (cases "fst x = k")
       case True
-      note i = True
-      show ?thesis        
-      proof (cases "fst x = k")
-        case True
-        with i show ?thesis by simp
-      next
-        case False
-        with goal1 i
-        have 
-          "x \<in> set (fst (ls_update k v 
-                           (ls ! bounded_hashcode_nat (length ls) k)))"
-          by auto
-        with 
-          ls_update_fst_set[
-            of k v "ls ! bounded_hashcode_nat (length ls) k"] 
-          False
-        have "x \<in> insert (k, v) 
-                    (set (ls ! bounded_hashcode_nat (length ls) k))" 
-          by auto
-        with False have "x \<in> set (ls ! bounded_hashcode_nat (length ls) k)"
-          by auto
-        with i goal1 assms[unfolded ht_hash_def] show ?thesis by simp
-      qed
+      with i show ?thesis by simp
     next
       case False
-      with goal1 have "x \<in> set (ls ! i)" by simp
-      with goal1 assms[unfolded ht_hash_def] show ?thesis by simp
+      with prems i
+      have
+        "x \<in> set (fst (ls_update k v
+                         (ls ! bounded_hashcode_nat (length ls) k)))"
+        by auto
+      with
+        ls_update_fst_set[
+          of k v "ls ! bounded_hashcode_nat (length ls) k"]
+        False
+      have "x \<in> insert (k, v)
+                  (set (ls ! bounded_hashcode_nat (length ls) k))"
+        by auto
+      with False have "x \<in> set (ls ! bounded_hashcode_nat (length ls) k)"
+        by auto
+      with i prems assms[unfolded ht_hash_def] show ?thesis by simp
     qed
-qed
+  next
+    case False
+    with prems have "x \<in> set (ls ! i)" by simp
+    with prems assms[unfolded ht_hash_def] show ?thesis by simp
+  qed
+  done
 
 
-
-lemma ht_distinct_update: 
+lemma ht_distinct_update:
   assumes "ht_distinct l"
   shows "ht_distinct (abs_update k v l)"
   unfolding ht_distinct_def abs_update_def
-proof (intro allI impI, simp)
-  case goal1 show ?case
+  apply (intro allI impI)
+  apply simp
+  subgoal premises prems for i
   proof (cases "i = bounded_hashcode_nat (length l) k")
     case True
-    with goal1 assms[unfolded ht_distinct_def]
+    with prems assms[unfolded ht_distinct_def]
     have "distinct (map fst (l ! bounded_hashcode_nat (length l) k))"
       by simp
-    from ls_update_distinct[OF this, of k v] True goal1
+    from ls_update_distinct[OF this, of k v] True prems
     show ?thesis by simp
   next
     case False
-    with goal1 assms[unfolded ht_distinct_def] show ?thesis by simp
+    with prems assms[unfolded ht_distinct_def] show ?thesis by simp
   qed
-qed
+  done
 
 
 lemma length_update:
@@ -345,46 +341,46 @@ lemma length_update:
   using assms
   by (simp add: abs_update_def)
 
-lemma ht_size_update1: 
+lemma ht_size_update1:
   assumes size: "ht_size l n"
   assumes i: "i < length l"
   assumes snd: "snd (ls_update k v (l ! i))"
   shows "ht_size (l[i := fst (ls_update k v (l!i))]) n"
 proof -
-  have "(map length (l[i := fst (ls_update k v (l ! i))])) 
+  have "(map length (l[i := fst (ls_update k v (l ! i))]))
     = map length l[i := length (fst (ls_update k v (l ! i)))]"
     by (simp add: map_update) also
-  from listsum_update_nat[of i "map length l", simplified, OF i, 
-    of "length (fst (ls_update k v (l ! i)))"] 
+  from listsum_update_nat[of i "map length l", simplified, OF i,
+    of "length (fst (ls_update k v (l ! i)))"]
     ls_update_length_snd_True[OF snd]
-  have 
+  have
     "listsum (map length l[i := length (fst (ls_update k v (l ! i)))])
     = listsum (map length l)" by simp
   finally show ?thesis using assms by (simp add: ht_size_def assms)
 qed
-    
-lemma ht_size_update2: 
+
+lemma ht_size_update2:
   assumes size: "ht_size l n"
   assumes i: "i < length l"
   assumes snd: "\<not> snd (ls_update k v (l ! i))"
   shows "ht_size (l[i := fst (ls_update k v (l!i))]) (Suc n)"
 proof -
-  have "(map length (l[i := fst (ls_update k v (l ! i))])) 
+  have "(map length (l[i := fst (ls_update k v (l ! i))]))
     = map length l[i := length (fst (ls_update k v (l ! i)))]"
     by (simp add: map_update) also
-  from listsum_update_nat[of i "map length l", simplified, OF i, 
-    of "length (fst (ls_update k v (l ! i)))"] 
+  from listsum_update_nat[of i "map length l", simplified, OF i,
+    of "length (fst (ls_update k v (l ! i)))"]
     ls_update_length_snd_False[OF snd]
-  have 
+  have
     "listsum (map length l[i := length (fst (ls_update k v (l ! i)))])
     = Suc (listsum (map length l))" by simp
   finally show ?thesis using assms by (simp add: ht_size_def assms)
-qed  
+qed
 
 
-lemma complete_ht_upd: "<is_hashtable l ht> ht_upd k v ht 
+lemma complete_ht_upd: "<is_hashtable l ht> ht_upd k v ht
   <is_hashtable (abs_update k v l)>"
-  unfolding ht_upd_def is_hashtable_def 
+  unfolding ht_upd_def is_hashtable_def
   apply (rule norm_pre_pure_rule)
   apply (rule bind_rule)
   apply (rule length_rule)
@@ -398,25 +394,23 @@ lemma complete_ht_upd: "<is_hashtable l ht> ht_upd k v ht
   apply (rule upd_rule)
   apply (simp add: bounded_hashcode_nat_bounds)
   apply (rule return_cons_rule)
-
-  apply (auto 
+  apply (auto
     simp add: ht_size_update1 ht_size_update2 bounded_hashcode_nat_bounds
               is_hashtable_def ht_hash_update[unfolded abs_update_def]
-              ht_distinct_update[unfolded abs_update_def] abs_update_def
-  )
+              ht_distinct_update[unfolded abs_update_def] abs_update_def)
   done
 
 text {* Alternative, more automatic proof *}
-lemma complete_ht_upd_alt_proof: 
+lemma complete_ht_upd_alt_proof:
   "<is_hashtable l ht> ht_upd k v ht <is_hashtable (abs_update k v l)>"
   unfolding ht_upd_def is_hashtable_def Let_def
   (* TODO: Is this huge simp-step really necessary? *)
   apply (sep_auto
     simp: ht_size_update1 ht_size_update2 bounded_hashcode_nat_bounds
               is_hashtable_def ht_hash_update[unfolded abs_update_def]
-              ht_distinct_update[unfolded abs_update_def] abs_update_def
-    )
+              ht_distinct_update[unfolded abs_update_def] abs_update_def)
   done
+
 
 subsection {* Delete *}
 
@@ -425,60 +419,62 @@ subsubsection {* Definition *}
 fun ls_delete :: "'k \<Rightarrow> ('k \<times> 'v) list \<Rightarrow> (('k \<times> 'v) list \<times> bool)" where
   "ls_delete k [] = ([], False)" |
   "ls_delete k ((l, w) # ls) = (
-    if k = l then 
-      (ls, True) 
-    else 
+    if k = l then
+      (ls, True)
+    else
       (let r = ls_delete k ls in ((l, w) # fst r, snd r)))"
 
-lemma ls_delete_snd_set:
-  "snd (ls_delete k l) \<longleftrightarrow> k \<in> set (map fst l)"
+lemma ls_delete_snd_set: "snd (ls_delete k l) \<longleftrightarrow> k \<in> set (map fst l)"
   by (induct l rule: ls_delete.induct) simp_all
 
-lemma ls_delete_fst_set:
-  "set (fst (ls_delete k l)) \<subseteq> set l"
-  apply (induct l rule: ls_delete.induct) 
+lemma ls_delete_fst_set: "set (fst (ls_delete k l)) \<subseteq> set l"
+  apply (induct l rule: ls_delete.induct)
   apply simp
-  by (auto simp add: Let_def)
+  apply (auto simp add: Let_def)
+  done
 
 lemma ls_delete_fst_map_set:
-  "distinct (map fst l) \<Longrightarrow> 
+  "distinct (map fst l) \<Longrightarrow>
   set (map fst (fst (ls_delete k l))) = (set (map fst l)) - {k}"
-  apply (induct l rule: ls_delete.induct) 
+  apply (induct l rule: ls_delete.induct)
   apply simp
-  by (auto simp add: Let_def)
+  apply (auto simp add: Let_def)
+  done
 
-lemma ls_delete_distinct: "distinct (map fst l) 
-  \<Longrightarrow> distinct (map fst (fst (ls_delete k l)))"
+lemma ls_delete_distinct: "distinct (map fst l) \<Longrightarrow> distinct (map fst (fst (ls_delete k l)))"
 proof (induct l rule: ls_delete.induct)
-  case goal1 thus ?case by simp
+  case 1 thus ?case by simp
 next
-  case goal2 show ?case
+  case (2 k l w ls) show ?case
   proof (cases "k = l")
     case True
-    with goal2 show ?thesis by simp
+    with 2 show ?thesis by simp
   next
     case False
-    with goal2 have d: "distinct (map fst (fst (ls_delete k ls)))" 
+    with 2 have d: "distinct (map fst (fst (ls_delete k ls)))"
       by simp
-    from goal2 have d2: "distinct (map fst ls)" by simp
-    from goal2(2) have "l \<notin> set (map fst ls)" by simp 
-    with False goal2 ls_delete_fst_map_set[OF d2, of k] 
+    from 2 have d2: "distinct (map fst ls)" by simp
+    from 2(2) have "l \<notin> set (map fst ls)" by simp
+    with False 2 ls_delete_fst_map_set[OF d2, of k]
     have "l \<notin> set (map fst (fst (ls_delete k ls)))"
-      apply (simp only:) by simp
+      by simp
     with d False show ?thesis by (simp add: Let_def)
   qed
 qed
 
-lemma ls_delete_length: 
+lemma ls_delete_length:
   "length (fst (ls_delete k l)) = (
-    if (k \<in> set (map fst l)) then 
-      (length l - 1) 
-    else 
+    if (k \<in> set (map fst l)) then
+      (length l - 1)
+    else
       length l)"
-  apply (induct l rule: ls_delete.induct)
-  apply (auto simp add: Let_def)
-  apply (case_tac ls)
-  by simp_all
+proof (induct l rule: ls_delete.induct)
+  case 1
+  then show ?case by simp
+next
+  case (2 k l w ls)
+  then show ?case by (cases ls) (auto simp add: Let_def)
+qed
 
 lemma ls_delete_length_snd_True:
   "snd (ls_delete k l) \<Longrightarrow> length (fst (ls_delete k l)) = length l - 1"
@@ -489,14 +485,14 @@ lemma ls_delete_length_snd_False:
   by (simp add: ls_delete_length ls_delete_snd_set)
 
 
-definition ht_delete 
-  :: "'k 
-    \<Rightarrow> ('k::{heap,hashable}, 'v::heap) hashtable 
-    \<Rightarrow> ('k, 'v) hashtable Heap" 
+definition ht_delete
+  :: "'k
+    \<Rightarrow> ('k::{heap,hashable}, 'v::heap) hashtable
+    \<Rightarrow> ('k, 'v) hashtable Heap"
   where
   "ht_delete k ht = do {
-      m \<leftarrow> Array.len (the_array ht); 
-      let i = bounded_hashcode_nat m k; 
+      m \<leftarrow> Array.len (the_array ht);
+      let i = bounded_hashcode_nat m k;
       l \<leftarrow> Array.nth (the_array ht) i;
       let l = ls_delete k l;
       Array.upd i (fst l) (the_array ht);
@@ -510,102 +506,103 @@ subsubsection {* Complete Correctness *}
 lemma ht_hash_delete:
   assumes "ht_hash ls"
   shows "ht_hash (
-    ls[bounded_hashcode_nat (length ls) k 
-      := fst (ls_delete k 
+    ls[bounded_hashcode_nat (length ls) k
+      := fst (ls_delete k
                (ls ! bounded_hashcode_nat (length ls) k)
              )
       ]
   )"
   unfolding ht_hash_def
-proof (intro allI ballI impI, simp)
-  case goal1 show ?case
-    proof (cases "i = bounded_hashcode_nat (length ls) k")
+  apply (intro allI ballI impI)
+  apply simp
+  subgoal premises prems for i x
+  proof (cases "i = bounded_hashcode_nat (length ls) k")
+    case i: True
+    show ?thesis
+    proof (cases "fst x = k")
       case True
-      note i = True
-      show ?thesis        
-      proof (cases "fst x = k")
-        case True
-        with i show ?thesis by simp
-      next
-        case False
-        with goal1 i
-        have 
-          "x \<in> set (fst (ls_delete k 
-                          (ls ! bounded_hashcode_nat (length ls) k)))"
-          by auto
-        with 
-          ls_delete_fst_set[
-            of k "ls ! bounded_hashcode_nat (length ls) k"] 
-          False
-        have "x \<in> (set (ls ! bounded_hashcode_nat (length ls) k))" by auto
-        with i goal1 assms[unfolded ht_hash_def] show ?thesis by simp
-      qed
+      with i show ?thesis by simp
     next
       case False
-      with goal1 have "x \<in> set (ls ! i)" by simp
-      with goal1 assms[unfolded ht_hash_def] show ?thesis by simp
+      with prems i
+      have
+        "x \<in> set (fst (ls_delete k
+                        (ls ! bounded_hashcode_nat (length ls) k)))"
+        by auto
+      with
+        ls_delete_fst_set[
+          of k "ls ! bounded_hashcode_nat (length ls) k"]
+        False
+      have "x \<in> (set (ls ! bounded_hashcode_nat (length ls) k))" by auto
+      with i prems assms[unfolded ht_hash_def] show ?thesis by simp
     qed
-qed
+  next
+    case False
+    with prems have "x \<in> set (ls ! i)" by simp
+    with prems assms[unfolded ht_hash_def] show ?thesis by simp
+  qed
+  done
 
-lemma ht_distinct_delete: 
+lemma ht_distinct_delete:
   assumes "ht_distinct l"
   shows "ht_distinct (
-    l[bounded_hashcode_nat (length l) k 
+    l[bounded_hashcode_nat (length l) k
       := fst (ls_delete k (l ! bounded_hashcode_nat (length l) k))])"
   unfolding ht_distinct_def
-proof (intro allI impI, simp)
-  case goal1 show ?case
+  apply (intro allI impI)
+  apply simp
+  subgoal premises prems for i
   proof (cases "i = bounded_hashcode_nat (length l) k")
     case True
-    with goal1 assms[unfolded ht_distinct_def]
+    with prems assms[unfolded ht_distinct_def]
     have "distinct (map fst (l ! bounded_hashcode_nat (length l) k))"
       by simp
-    from ls_delete_distinct[OF this, of k] True goal1
+    from ls_delete_distinct[OF this, of k] True prems
     show ?thesis by simp
   next
     case False
-    with goal1 assms[unfolded ht_distinct_def] show ?thesis by simp
+    with prems assms[unfolded ht_distinct_def] show ?thesis by simp
   qed
-qed
+  done
 
-lemma ht_size_delete1: 
+lemma ht_size_delete1:
   assumes size: "ht_size l n"
   assumes i: "i < length l"
   assumes snd: "snd (ls_delete k (l ! i))"
   shows "ht_size (l[i := fst (ls_delete k (l!i))]) (n - 1)"
 proof -
-  have "(map length (l[i := fst (ls_delete k (l ! i))])) 
+  have "(map length (l[i := fst (ls_delete k (l ! i))]))
     = map length l[i := length (fst (ls_delete k (l ! i)))]"
     by (simp add: map_update) also
-  from listsum_update_nat[of i "map length l", simplified, OF i, 
-    of "length (fst (ls_delete k (l ! i)))"] 
+  from listsum_update_nat[of i "map length l", simplified, OF i,
+    of "length (fst (ls_delete k (l ! i)))"]
     ls_delete_length_snd_True[OF snd] snd
   have "listsum (map length l[i := length (fst (ls_delete k (l ! i)))])
     = listsum (map length l) - 1"
     by (cases "length (l ! i)") (simp_all add: ls_delete_snd_set)
   finally show ?thesis using assms by (simp add: ht_size_def assms)
 qed
-    
-lemma ht_size_delete2: 
+
+lemma ht_size_delete2:
   assumes size: "ht_size l n"
   assumes i: "i < length l"
   assumes snd: "\<not> snd (ls_delete k (l ! i))"
   shows "ht_size (l[i := fst (ls_delete k (l!i))]) n"
 proof -
-  have "(map length (l[i := fst (ls_delete k (l ! i))])) 
+  have "(map length (l[i := fst (ls_delete k (l ! i))]))
     = map length l[i := length (fst (ls_delete k (l ! i)))]"
     by (simp add: map_update) also
-  from listsum_update_nat[of i "map length l", simplified, OF i, 
-    of "length (fst (ls_delete k (l ! i)))"] 
+  from listsum_update_nat[of i "map length l", simplified, OF i,
+    of "length (fst (ls_delete k (l ! i)))"]
     ls_delete_length_snd_False[OF snd]
   have "listsum (map length l[i := length (fst (ls_delete k (l ! i)))])
     = listsum (map length l)" by simp
   finally show ?thesis using assms by (simp add: ht_size_def assms)
-qed  
+qed
 
 
-lemma complete_ht_delete: "<is_hashtable l ht> ht_delete k ht 
-  <is_hashtable (l[bounded_hashcode_nat (length l) k 
+lemma complete_ht_delete: "<is_hashtable l ht> ht_delete k ht
+  <is_hashtable (l[bounded_hashcode_nat (length l) k
     := fst (ls_delete k (l ! bounded_hashcode_nat (length l) k))])>"
   unfolding ht_delete_def is_hashtable_def
   apply (rule norm_pre_pure_rule)
@@ -621,47 +618,45 @@ lemma complete_ht_delete: "<is_hashtable l ht> ht_delete k ht
   apply (rule upd_rule)
   apply (simp add: bounded_hashcode_nat_bounds)
   apply (rule return_cons_rule)
-
-  apply (auto 
+  apply (auto
     simp add: ht_size_delete1 ht_size_delete2 bounded_hashcode_nat_bounds
-              is_hashtable_def ht_hash_delete ht_distinct_delete 
-              )
-
-  using ht_size_delete1[OF _ bounded_hashcode_nat_bounds[of "length l" k],
-    of "the_size ht"]
-  by simp
+              is_hashtable_def ht_hash_delete ht_distinct_delete)
+  using ht_size_delete1[OF _ bounded_hashcode_nat_bounds[of "length l" k], of "the_size ht"]
+  apply simp
+  done
 
 text {* Alternative, more automatic proof *}
-lemma "<is_hashtable l ht> ht_delete k ht 
-  <is_hashtable (l[bounded_hashcode_nat (length l) 
+lemma "<is_hashtable l ht> ht_delete k ht
+  <is_hashtable (l[bounded_hashcode_nat (length l)
     k := fst (ls_delete k (l ! bounded_hashcode_nat (length l) k))])>"
   unfolding ht_delete_def is_hashtable_def Let_def
   using ht_size_delete1[OF _ bounded_hashcode_nat_bounds[of "length l" k],
     of "the_size ht"]
   apply (sep_auto simp:
     ht_size_delete1 ht_size_delete2 bounded_hashcode_nat_bounds
-    is_hashtable_def ht_hash_delete ht_distinct_delete
-    )
+    is_hashtable_def ht_hash_delete ht_distinct_delete)
   done
 
 
 subsection {* Re-Hashing *}
+
 subsubsection {* Auxiliary Functions *}
 
 text {* \paragraph{Insert List} *}
-fun ht_insls 
-  :: "('k \<times> 'v) list 
-    \<Rightarrow> ('k::{heap,hashable}, 'v::heap) hashtable 
-    \<Rightarrow> ('k, 'v::heap) hashtable Heap" 
+fun ht_insls
+  :: "('k \<times> 'v) list
+    \<Rightarrow> ('k::{heap,hashable}, 'v::heap) hashtable
+    \<Rightarrow> ('k, 'v::heap) hashtable Heap"
   where
   "ht_insls [] ht = return ht" |
   "ht_insls ((k, v) # l) ht = do { h \<leftarrow> ht_upd k v ht; ht_insls l h }"
 
 text "Abstract version"
-fun ls_insls :: "('k::hashable \<times> 'v) list 
-  \<Rightarrow> ('k \<times> 'v) list list \<Rightarrow> ('k \<times> 'v) list list" where
+fun ls_insls :: "('k::hashable \<times> 'v) list
+  \<Rightarrow> ('k \<times> 'v) list list \<Rightarrow> ('k \<times> 'v) list list"
+where
   "ls_insls [] l = l" |
-  "ls_insls ((k, v) # ls) l = 
+  "ls_insls ((k, v) # ls) l =
     ls_insls ls (abs_update k v l)"
 
 lemma ht_hash_ls_insls:
@@ -670,60 +665,64 @@ lemma ht_hash_ls_insls:
   using assms
   apply (induct l rule: ls_insls.induct)
   apply simp
-  by (simp add: ht_hash_update)  
+  apply (simp add: ht_hash_update)
+  done
 
-lemma ht_distinct_ls_insls: 
+lemma ht_distinct_ls_insls:
   assumes "ht_distinct l"
   shows "ht_distinct (ls_insls ls l)"
   using assms
   apply (induct l rule: ls_insls.induct)
   apply simp
-  by (simp add: ht_distinct_update)    
+  apply (simp add: ht_distinct_update)
+  done
 
 lemma length_ls_insls:
   assumes "1 < length l"
   shows "1 < length (ls_insls ls l)"
   using assms
-  apply (induct l rule: ls_insls.induct)
-  apply simp
-proof -
-  case goal1
-  from goal1(1)[OF length_update[OF goal1(2), of k v]] show ?case
+proof (induct l rule: ls_insls.induct)
+  case 1
+  then show ?case by simp
+next
+  case (2 k v ls l)
+  from 2(1)[OF length_update[OF 2(2), of k v]] show ?case
     by simp
 qed
 
-lemma complete_ht_insls: 
+lemma complete_ht_insls:
   "<is_hashtable ls ht> ht_insls xs ht <is_hashtable (ls_insls xs ls)>"
 proof (induct xs arbitrary: ls ht)
-  case goal1 show ?case by (auto intro: return_cons_rule)[]
+  case Nil
+  show ?case by (auto intro: return_cons_rule)
 next
-  case (goal2 x xs ls ht)
-  note IV = goal2
+  case (Cons x xs)
   show ?case
   proof (cases x)
-    case (goal1 k v)
-    thus ?case
+    case (Pair k v)
+    then show ?thesis
       apply simp
       apply (rule bind_rule)
       apply (rule complete_ht_upd)
-      by (simp add: IV)
+      apply (simp add: Cons)
+      done
   qed
 qed
 
 text {* \paragraph{Copy} *}
-fun ht_copy :: "nat \<Rightarrow> ('k::{heap,hashable}, 'v::heap) hashtable 
-  \<Rightarrow> ('k, 'v) hashtable \<Rightarrow> ('k, 'v) hashtable Heap" 
+fun ht_copy :: "nat \<Rightarrow> ('k::{heap,hashable}, 'v::heap) hashtable
+  \<Rightarrow> ('k, 'v) hashtable \<Rightarrow> ('k, 'v) hashtable Heap"
   where
   "ht_copy 0 src dst = return dst" |
-  "ht_copy (Suc n) src dst = do { 
-    l \<leftarrow> Array.nth (the_array src) n; 
-    ht \<leftarrow> ht_insls l dst; 
-    ht_copy n src ht 
+  "ht_copy (Suc n) src dst = do {
+    l \<leftarrow> Array.nth (the_array src) n;
+    ht \<leftarrow> ht_insls l dst;
+    ht_copy n src ht
   }"
 
 text "Abstract version"
-fun ls_copy :: "nat \<Rightarrow> ('k::hashable \<times> 'v) list list 
-  \<Rightarrow> ('k \<times> 'v) list list \<Rightarrow> ('k \<times> 'v) list list" 
+fun ls_copy :: "nat \<Rightarrow> ('k::hashable \<times> 'v) list list
+  \<Rightarrow> ('k \<times> 'v) list list \<Rightarrow> ('k \<times> 'v) list list"
   where
   "ls_copy 0 ss ds = ds" |
   "ls_copy (Suc n) ss ds = ls_copy n ss (ls_insls (ss ! n) ds)"
@@ -734,147 +733,139 @@ lemma ht_hash_ls_copy:
   using assms
   apply (induct n arbitrary: l)
   apply simp
-  by (simp add: ht_hash_ls_insls)
+  apply (simp add: ht_hash_ls_insls)
+  done
 
-lemma ht_distinct_ls_copy: 
+lemma ht_distinct_ls_copy:
   assumes "ht_distinct l"
-  shows "ht_distinct (ls_copy n ss l)"  
+  shows "ht_distinct (ls_copy n ss l)"
   using assms
   apply (induct n arbitrary: l)
   apply simp
-  by (simp add: ht_distinct_ls_insls)
+  apply (simp add: ht_distinct_ls_insls)
+  done
 
 lemma length_ls_copy:
   assumes "1 < length l"
-  shows "1 < length (ls_copy n ss l)"  
+  shows "1 < length (ls_copy n ss l)"
   using assms
-  apply (induct n arbitrary: l)
-  apply simp
-proof -
-  case goal1
-  from goal1(1)[OF length_ls_insls[OF goal1(2)]] show ?case by simp
+proof (induct n arbitrary: l)
+  case 0
+  then show ?case by simp
+next
+  case (Suc n)
+  from Suc(1)[OF length_ls_insls[OF Suc(2)]] show ?case by simp
 qed
 
-lemma complete_ht_copy: "n \<le> List.length ss \<Longrightarrow> 
-  <is_hashtable ss src * is_hashtable ds dst> 
-  ht_copy n src dst 
+lemma complete_ht_copy: "n \<le> List.length ss \<Longrightarrow>
+  <is_hashtable ss src * is_hashtable ds dst>
+  ht_copy n src dst
   <\<lambda>r. is_hashtable ss src * is_hashtable (ls_copy n ss ds) r>"
 proof (induct n arbitrary: ds dst)
-  case goal1
+  case 0
   show ?case by (auto intro!: return_cons_rule)
 next
-  case goal2
-  from goal2 have n: "n < length ss" by simp
-  hence "n \<le> length ss" by simp
-  note IV = goal2(1)[OF this]
+  case (Suc n)
+  then have n: "n < length ss" by simp
+  then have "n \<le> length ss" by simp
+  note IH = Suc(1)[OF this]
   show ?case
     apply simp
     apply (rule bind_rule)
     apply (rule frame_rule)
-    apply (subgoal_tac "<is_hashtable ss src> 
-      Array.nth (the_array src) n 
+    apply (subgoal_tac "<is_hashtable ss src>
+      Array.nth (the_array src) n
       <\<lambda>r. is_hashtable ss src * \<up>(r = ss ! n)>")
     apply simp
     apply (simp add: is_hashtable_def)
     apply (auto intro!: nth_rule simp add: n)[]
-    apply (clarsimp simp: norm_assertion_simps)
+    apply clarsimp
     apply (rule bind_rule)
     apply (rule frame_rule_left)
     apply (rule complete_ht_insls)
-    apply (simp add: IV)
+    apply (simp add: IH)
     done
 qed
 
 text {* Alternative, more automatic proof *}
-lemma complete_ht_copy_alt_proof: "n \<le> List.length ss \<Longrightarrow> 
-  <is_hashtable ss src * is_hashtable ds dst> 
-  ht_copy n src dst 
+lemma complete_ht_copy_alt_proof: "n \<le> List.length ss \<Longrightarrow>
+  <is_hashtable ss src * is_hashtable ds dst>
+  ht_copy n src dst
   <\<lambda>r. is_hashtable ss src * is_hashtable (ls_copy n ss ds) r>"
 proof (induct n arbitrary: ds dst)
-  case goal1
+  case 0
   show ?case by (sep_auto)
 next
-  case goal2
-  from goal2 have N_LESS: "n < length ss" by simp
-  hence N_LE: "n \<le> length ss" by simp
-  note IV = goal2(1)[OF this]
+  case (Suc n)
+  then have N_LESS: "n < length ss" by simp
+  then have N_LE: "n \<le> length ss" by simp
+  note IH = Suc(1)[OF this]
   show ?case
-    by (sep_auto 
-      simp: N_LESS N_LE 
-      heap: complete_ht_insls IV)
+    by (sep_auto simp: N_LESS N_LE heap: complete_ht_insls IH)
 qed
-    
-definition ht_rehash 
+
+definition ht_rehash
   :: "('k::{heap,hashable}, 'v::heap) hashtable \<Rightarrow> ('k, 'v) hashtable Heap"
   where
-  "ht_rehash ht = do { 
-    n \<leftarrow> Array.len (the_array ht); 
-    h \<leftarrow> ht_new_sz (2 * n); 
+  "ht_rehash ht = do {
+    n \<leftarrow> Array.len (the_array ht);
+    h \<leftarrow> ht_new_sz (2 * n);
     ht_copy n ht h
   }"
 
 text "Operation on Abstraction"
-definition ls_rehash 
-  :: "('k::hashable \<times> 'v) list list \<Rightarrow> ('k \<times> 'v) list list" 
-  where "ls_rehash l 
-  = ls_copy (List.length l) l (replicate (2 * length l) [])"
+definition ls_rehash :: "('k::hashable \<times> 'v) list list \<Rightarrow> ('k \<times> 'v) list list"
+  where "ls_rehash l = ls_copy (List.length l) l (replicate (2 * length l) [])"
 
-lemma ht_hash_ls_rehash:
-  shows "ht_hash (ls_rehash l)"
+lemma ht_hash_ls_rehash: "ht_hash (ls_rehash l)"
   by (simp add: ht_hash_ls_copy ls_rehash_def)
 
-lemma ht_distinct_ls_rehash: 
-  shows "ht_distinct (ls_rehash l)"  
+lemma ht_distinct_ls_rehash: "ht_distinct (ls_rehash l)"
   by (simp add: ht_distinct_ls_copy ls_rehash_def)
 
 lemma length_ls_rehash:
   assumes "1 < length l"
   shows "1 < length (ls_rehash l)"
-  using assms
 proof -
-  case goal1
-  hence "1 < length (replicate (2 * length l) [])" by simp
-  from length_ls_copy[OF this, of "length l" l] show ?case 
+  from assms have "1 < length (replicate (2 * length l) [])" by simp
+  from length_ls_copy[OF this, of "length l" l] show ?thesis
     by (simp add: ls_rehash_def)
 qed
 
-lemma ht_imp_len: 
-  "is_hashtable l ht \<Longrightarrow>\<^sub>A is_hashtable l ht * \<up>(length l > 0)"
+lemma ht_imp_len: "is_hashtable l ht \<Longrightarrow>\<^sub>A is_hashtable l ht * \<up>(length l > 0)"
   unfolding is_hashtable_def
   by sep_auto
 
-lemma complete_ht_rehash: 
-  "<is_hashtable l ht> ht_rehash ht 
+lemma complete_ht_rehash:
+  "<is_hashtable l ht> ht_rehash ht
   <\<lambda>r. is_hashtable l ht * is_hashtable (ls_rehash l) r>"
   apply (rule cons_pre_rule[OF ht_imp_len])
   unfolding ht_rehash_def
-  apply (sep_auto 
-    heap: complete_ht_new_sz
-  )
-  apply (cases l, simp_all) []
+  apply (sep_auto heap: complete_ht_new_sz)
+  apply (cases l; simp)
   apply (sep_auto heap: complete_ht_copy simp: ls_rehash_def)
   done
 
 definition load_factor :: nat -- "in percent"
   where "load_factor = 75"
 
-definition ht_update 
-  :: "'k::{heap,hashable} \<Rightarrow> 'v::heap \<Rightarrow> ('k, 'v) hashtable 
-  \<Rightarrow> ('k, 'v) hashtable Heap" 
+definition ht_update
+  :: "'k::{heap,hashable} \<Rightarrow> 'v::heap \<Rightarrow> ('k, 'v) hashtable
+  \<Rightarrow> ('k, 'v) hashtable Heap"
   where
-  "ht_update k v ht = do { 
-    m \<leftarrow> Array.len (the_array ht); 
-    ht \<leftarrow> (if m * load_factor \<le> (the_size ht) * 100 then 
-        ht_rehash ht 
+  "ht_update k v ht = do {
+    m \<leftarrow> Array.len (the_array ht);
+    ht \<leftarrow> (if m * load_factor \<le> (the_size ht) * 100 then
+        ht_rehash ht
       else return ht);
-    ht_upd k v ht 
+    ht_upd k v ht
   }"
 
 
-lemma complete_ht_update_normal: 
-  "\<not> length l * load_factor \<le> (the_size ht)* 100 \<Longrightarrow> 
-  <is_hashtable l ht> 
-  ht_update k v ht 
+lemma complete_ht_update_normal:
+  "\<not> length l * load_factor \<le> (the_size ht)* 100 \<Longrightarrow>
+  <is_hashtable l ht>
+  ht_update k v ht
   <is_hashtable (abs_update k v l)>"
   unfolding ht_update_def
   apply (sep_auto simp: is_hashtable_def)
@@ -883,26 +874,28 @@ lemma complete_ht_update_normal:
   apply (simp add: complete_ht_upd)
   done
 
-lemma complete_ht_update_rehash: 
-  "length l * load_factor \<le> (the_size ht)* 100 \<Longrightarrow> 
-  <is_hashtable l ht> 
-  ht_update k v ht 
-  <\<lambda>r. is_hashtable l ht 
+lemma complete_ht_update_rehash:
+  "length l * load_factor \<le> (the_size ht)* 100 \<Longrightarrow>
+  <is_hashtable l ht>
+  ht_update k v ht
+  <\<lambda>r. is_hashtable l ht
     * is_hashtable (abs_update k v (ls_rehash l)) r>"
   unfolding ht_update_def
   by (sep_auto heap: complete_ht_rehash complete_ht_upd)
 
+
 subsection {* Conversion to List *}
-definition ht_to_list :: 
+
+definition ht_to_list ::
   "('k::heap, 'v::heap) hashtable \<Rightarrow> ('k \<times> 'v) list Heap" where
-  "ht_to_list ht = do { 
-    l \<leftarrow> (Array.freeze (the_array ht)); 
-    return (concat l) 
+  "ht_to_list ht = do {
+    l \<leftarrow> (Array.freeze (the_array ht));
+    return (concat l)
   }"
 
-lemma complete_ht_to_list: "<is_hashtable l ht> ht_to_list ht 
+lemma complete_ht_to_list: "<is_hashtable l ht> ht_to_list ht
   <\<lambda>r. is_hashtable l ht * \<up>(r = concat l)>"
   unfolding ht_to_list_def is_hashtable_def
   by sep_auto
-  
+
 end
